\documentclass[12pt]{article}
\usepackage[utf8]{inputenc}
\usepackage{amsmath,amssymb,amsthm}
\newenvironment{note}{\paragraph{NOTE:}}{}
\newenvironment{field}{\paragraph{field:}}{}
%\newenvironment{tags}{\paragraph{tags:}}{}
\newcommand*{\tags}[1]{\paragraph{tags: }#1}


\begin{document}

%%start_tag Calculus

\tags{Calculus}

\begin{note}
  \begin{field}
    $\int_0^\infty e^{-x^2/2} = $
  \end{field}
  \begin{field}
    $\int_0^\infty e^{-x^2/2} = \sqrt{\pi/2}$
  \end{field}
\end{note}


\begin{note}
  \begin{field}
    $\int_0^\infty x^{a-1}e^{-x/b} = $
  \end{field}
  \begin{field}
    $\int_0^\infty x^{a-1}e^{-x/b} = \Gamma(a)b^a$
  \end{field}
\end{note}

\begin{note}
  \begin{field}
    $\int_0^1 x^{a - 1}(1 - x)^{b-1} = $
  \end{field}
  \begin{field}
    $\int_0^1 x^{a - 1}(1 - x)^{b-1} = \frac{\Gamma(a)\Gamma(b)}{\Gamma(a + b)}$
  \end{field}
\end{note}

\begin{note}
  \begin{field}
    $\log(x) = y , x = $
  \end{field}
  \begin{field}
    $\log(x) = y , x = e^y$
  \end{field}
\end{note}

\begin{note}
  \begin{field}
    $\lim_{x \to \infty}( 1 + \frac{a}{x})^x = $
  \end{field}
    \begin{field}
      $\lim_{x \to \infty}( 1 + \frac{a}{x})^x = e^a$
    \end{field}
\end{note}

\begin{note}
  \begin{field}
    $\lim_{x \to \infty}( 1 + \frac{a}{x})^x = e^a$
  \end{field}
  \begin{field}
    $\lim_{x \to \infty}( 1 + \frac{a}{x})^x = $
  \end{field}
\end{note}

\begin{note}
  \begin{field}
    $\frac{d}{dx}f(g(x)) = $
  \end{field}
  \begin{field}
    $\frac{d}{dx}f(g(x)) = f'(g(x))g'(x)$ (Chain rule)
  \end{field}
\end{note}

\begin{note}
  \begin{field}
    $\frac{d}{dx} \int_{a}^x f(t)dt = $
  \end{field}
  \begin{field}
    $\frac{d}{dx} \int_{a}^x f(t)dt = f(x)$ (fundamental theorem of calculus )
  \end{field}
\end{note}


\begin{note}
  \begin{field}
    $\int_a^b u dv = $

    ex: $\int x e^{-x}$
  \end{field}
  \begin{field}
    $\int_a^b u dv = uv|_a^b - \int_a^b v du $

    ex: $u = x, dv = e^{-x}, du = dx, v = -e^{-x}$
    \begin{align*}
      \int x e^{-x} &= -x e^{-x} + \int e^{-x} \\
      &= -x e^{-x}  -e^{-x} + c
    \end{align*}
  \end{field}
\end{note}

\begin{note}
  \begin{field}
    $\sum_{k=0}^\infty \frac{x^k}{k!} = $
  \end{field}
  \begin{field}
    $\sum_{k=0}^\infty \frac{x^k}{k!} = e^x$
  \end{field}
\end{note}


\begin{note}
  \begin{field}
    $e^x = $
  \end{field}
  \begin{field}
    $e^x = \sum_{k=0}^\infty \frac{x^k}{k!}$
  \end{field}
\end{note}

\begin{note}
  \begin{field}
    $\sum_{k=0}^\infty x^k = $
  \end{field}
  \begin{field}
    $\sum_{k=0}^\infty x^k = \frac{1}{1-x}$ for $|x| < 1$
  \end{field}
\end{note}


\begin{note}
  \begin{field}
    $\sum_{k=0}^n x^k =$
  \end{field}
  \begin{field}
    $\sum_{k=0}^n x^k = \frac{1 - x^{n+1}}{1-x}$ for $x \neq 1$
  \end{field}
\end{note}

\begin{note}
  \begin{field}
    $\lim_{x \to -\infty} e^{-x} = $
  \end{field}
  \begin{field}
    $\lim_{x \to -\infty} e^{-x} = \infty$
  \end{field}
\end{note}

\begin{note}
  \begin{field}
    $\lim_{x \to \infty} e^{-x} = $
  \end{field}
  \begin{field}
    $\lim_{x \to -\infty} e^{-x} = 0$
  \end{field}
\end{note}

\begin{note}
  \begin{field}
    $$ (fg)' = $$
  \end{field}
  \begin{field}
    $$ (fg)' = f'g + g'f$$ (product rule )
  \end{field}
\end{note}

\begin{note}
  \begin{field}
    $\frac{d}{dx} x^n = $
  \end{field}
  \begin{field}
    $\frac{d}{dx} x^n = nx^{n-1}$
  \end{field}
\end{note}

\begin{note}
  \begin{field}
    $\frac{d}{dx} a^x = $
  \end{field}
  \begin{field}
    $\frac{d}{dx} a^x = a^x ln(a)$
  \end{field}
\end{note}

\begin{note}
  \begin{field}
    $\frac{d}{dx} ln(x) = $
  \end{field}
  \begin{field}
    $\frac{d}{dx} ln(x) = \frac{1}{x}$
  \end{field}
\end{note}

\begin{note}
  \begin{field}
    $\frac{d}{dx} (f(x))^n = $
  \end{field}
  \begin{field}
    $\frac{d}{dx} (f(x))^n = n(f(x))^{n-1}f'(x)$
  \end{field}
\end{note}

\begin{note}
  \begin{field}
    $ \frac{d}{dx} ln(f(x)) = $
  \end{field}
  \begin{field}
    $ \frac{d}{dx} ln(f(x)) = \frac{f'(x)}{f(x)}$
  \end{field}
\end{note}

\begin{note}
  \begin{field}
    $\frac{d}{dx} e^{f(x)} = $
  \end{field}
  \begin{field}
    $\frac{d}{dx} e^{f(x)} = f'(x)e^{f(x)}$
  \end{field}
\end{note}

\begin{note}
  \begin{field}
    $\int x^n = $
  \end{field}
  \begin{field}
    $\int x^n = \frac{1}{n+1}x^{n+1}$
  \end{field}
\end{note}

\begin{note}
  \begin{field}
    $\int \frac{1}{x} = $
  \end{field}
  \begin{field}
    $\int \frac{1}{x} = ln(|x|)$
  \end{field}
\end{note}

\begin{note}
  \begin{field}
    $\int \frac{1}{ax + b} = $
  \end{field}
  \begin{field}
    $\int \frac{1}{ax + b} = \frac{1}{a}ln(|ax + b|)$
  \end{field}
\end{note}

\begin{note}
  \begin{field}
    $\int e^{cx} = $
  \end{field}
  \begin{field}
    $\int e^{cx} = \frac{1}{c}e^{cx}$
  \end{field}
\end{note}

\begin{note}
  \begin{field}
    $\int x e^{-cx^2} = $
  \end{field}
  \begin{field}
    $\int x e^{-cx^2} = -\frac{1}{2c}e^{-cx^2}$
  \end{field}
\end{note}

\begin{note}
  \begin{field}
    U substitution:

    example; $\int_1^2 5x^2\cos(x^3)$
  \end{field}
  \begin{field}
    $\int_a^bf(g(x))g'(x) = \int_{g(a)}^g(b) f(u)du$

    Where $u = g(x), du = g' dx$

    Ex: $u = x^3, du = 3x^2, x^2 du = 1/3 du$
    $\int_1^2 5x^2\cos(x^3) = \int_{1}^8 5/3 \cos(u)du$

  \end{field}
\end{note}

\begin{note}
  \begin{field}
    $\Gamma(a) = $
  \end{field}
  \begin{field}
    $\int_0^\infty t^{a-1}e^{-t}dt $
  \end{field}
\end{note}

\begin{note}
  \begin{field}
    $\int_0^\infty t^{a-1}e^{-t}dt $
  \end{field}
  \begin{field}
    $= \Gamma(a) $
  \end{field}
\end{note}


\begin{note}
  \begin{field}
    $\Gamma(a + 1) = $
  \end{field}
  \begin{field}
    $\Gamma(a + 1) = a\Gamma(a)$
  \end{field}
\end{note}

\begin{note}
  \begin{field}
    $\Gamma(n) = $
  \end{field}
  \begin{field}
    $\Gamma(n) = (n-1)!$ (for $n$ an integer)
  \end{field}
\end{note}

\begin{note}
  \begin{field}
    $\Gamma(1/2) = $
  \end{field}
  \begin{field}
    $\Gamma(1/2) = \sqrt{\pi}$
  \end{field}
\end{note}

\begin{note}
  \begin{field}
    $\Gamma(1) = $
  \end{field}
  \begin{field}
    $\Gamma(1) = 1$
  \end{field}
\end{note}


%%end_tag




\end{document}
